Binary counter with offset

theories/examples/counter_binary_preamble.v
@@ -18,11 +18,18 @@ Section counter_example_preamble.
   Definition counter_right_instrs :=
     decr_instrs ++ read_neg_instrs.
 
+  Variable offset: nat.
+  Definition counter_offset_instrs :=
+    offset_incr_instrs ++ offset_read_instrs offset.
+
   Definition counter_left a :=
     ([∗ list] a_i;w ∈ a;counter_left_instrs, a_i ↦ₐ w )%I.
 
   Definition counter_right a :=
     ([∗ list] a_i;w ∈ a;counter_right_instrs, a_i ↣ₐ w )%I.
+
+  Definition counter_offset a :=
+    ([∗ list] a_i;w ∈ a;counter_offset_instrs, a_i ↣ₐ w )%I.
 
   Definition counter_left_instrs_length : Z :=
     Eval cbv in (length (counter_left_instrs)).
@@ -37,6 +44,13 @@ Section counter_example_preamble.
     Eval cbv in (length (decr_instrs)).
   Definition read_neg_instrs_length : Z :=
     Eval cbv in (length (read_neg_instrs)).
+
+  Definition counter_offset_instrs_length : Z :=
+    Eval cbv in (length (counter_offset_instrs)).
+  Definition offset_incr_instrs_length : Z :=
+    Eval cbv in (length (offset_incr_instrs)).
+  Definition offset_read_instrs_length : Z :=
+    Eval cbv in (length (offset_read_instrs offset)).
 
   (* [f_m] is the offset of the malloc capability *)
   (* [offset_to_counter] is the offset between the [move_r r_t1 PC] instruction
@@ -90,10 +104,38 @@ Section counter_example_preamble.
     move_z r_t9 0;
     jmp r_t0].
 
+  (* [f_m] is the offset of the malloc capability *)
+  (* [offset_to_counter] is the offset between the [move_r r_t1 PC] instruction
+  and the code of the specification counter, which will be the concatenation of: decr;read_neg *)
+  Definition counter_offset_preamble_instrs (f_m offset_to_counter: Z) :=
+    malloc_instrs f_m 1%nat ++
+    [store_z r_t1 offset;
+    move_r r_t2 r_t1;
+    move_r r_t1 PC;
+    move_r r_t8 r_t2; (* we keep a copy of the capability for the other closures *)
+    move_r r_t9 r_t1; (* same for PC *)
+    (* closure for incr *)
+    lea_z r_t1 offset_to_counter] ++
+    crtcls_instrs f_m ++
+    [move_r r_t10 r_t1;
+    move_r r_t2 r_t8;
+    move_r r_t1 r_t9;
+    (* closure for read *)
+    lea_z r_t1 (offset_to_counter + offset_incr_instrs_length)] ++
+    crtcls_instrs f_m ++
+    (* cleanup *)
+    [move_r r_t2 r_t10;
+    move_z r_t10 0;
+    move_z r_t8 0;
+    move_z r_t9 0;
+    jmp r_t0].
+
   Definition counter_left_preamble f_m offset_to_counter ai :=
     ([∗ list] a_i;w_i ∈ ai;(counter_left_preamble_instrs f_m offset_to_counter), a_i ↦ₐ w_i)%I.
   Definition counter_right_preamble f_m offset_to_counter ai :=
     ([∗ list] a_i;w_i ∈ ai;(counter_right_preamble_instrs f_m offset_to_counter), a_i ↣ₐ w_i)%I.
+  Definition counter_offset_preamble f_m offset_to_counter ai :=
+    ([∗ list] a_i;w_i ∈ ai;(counter_offset_preamble_instrs f_m offset_to_counter), a_i ↣ₐ w_i)%I.
 
   (* Compute the offset from the start of the program to the move_r r_t1 PC
      instruction. Will be used later to compute [offset_to_awkward]. *)
@@ -255,6 +297,119 @@ Section counter_example_preamble.
     { iNext. iIntros (?) "HH". iIntros (->). iApply "HH". eauto. }
   Qed.
 
+
+  Lemma incr_offset_closure_valid incr_prog offset_prog
+        restc srestc count_incroffN countN count_clsN
+        b_cls e_cls (* incr/decr closure *)
+        b_cls' e_cls' (* read/read_neg closure *)
+        pc_p pc_b pc_e counter_first counter_end linkc (* left PC values *)
+        pcs_p pcs_b pcs_e scounter_first scounter_end slinkc (* right PC values *)
+        b_cell e_cell (* left counter *)
+        bs_cell es_cell (* right counter *):
+
+    pc_p ≠ E → pcs_p ≠ E →
+
+    contiguous_between incr_prog counter_first linkc →
+    contiguous_between offset_prog scounter_first slinkc →
+    isCorrectPC_range pc_p pc_b pc_e counter_first counter_end →
+    isCorrectPC_range pcs_p pcs_b pcs_e scounter_first scounter_end →
+
+    contiguous_between restc linkc counter_end →
+    contiguous_between srestc slinkc scounter_end →
+    (b_cell + 1)%a = Some e_cell →
+    (bs_cell + 1)%a = Some es_cell →
+    nclose specN ## ↑countN →
+
+    ⊢ (spec_ctx -∗ inv countN (offset_counter_inv offset b_cell bs_cell) -∗
+     na_inv logrel_nais count_incroffN (incr_left incr_prog ∗ offset_right offset_prog) -∗
+     na_inv logrel_nais count_clsN (cls_inv b_cls e_cls b_cls' e_cls' (WCap pc_p pc_b pc_e counter_first)
+                                            (WCap pc_p pc_b pc_e linkc) (WCap RWX b_cell e_cell b_cell)
+
+                                            (WCap pcs_p pcs_b pcs_e scounter_first) (WCap pcs_p pcs_b pcs_e slinkc)
+                                            (WCap RWX bs_cell es_cell bs_cell)) -∗
+     na_own logrel_nais ⊤ -∗
+    interp (WCap E b_cls e_cls b_cls,WCap E b_cls e_cls b_cls))%I.
+  Proof.
+    iIntros (Hnp Hnps Hcont_incr Hcont_decr Hvpc_counter Hvspc_counter Hcont_restc Hcont_srestc Hbe_cell Hbes_cell Hnclose)
+            "#Hspec #Hcounter_inv #Hincr #Hcls_inv HnaI".
+    rewrite /interp fixpoint_interp1_eq /=. iSplit;auto.
+    iIntros (r') "". iNext. iModIntro.
+    iIntros "(#Hr_valid & Hregs' & Hsegs' & HnaI & Hj)". destruct r' as [r1' r2']. simpl.
+    iDestruct (interp_reg_eq _ _ (WCap RX b_cls e_cls b_cls) with "Hr_valid") as %Heq.
+    iDestruct "Hr_valid" as "[Hr'_full Hr'_valid]"; iDestruct "Hr'_full" as %Hr'_full.
+    assert (∀ x : RegName, is_Some (r1' !! x)) as Hr'_full_left;[intros x; destruct Hr'_full with x;eauto|].
+    assert (∀ x : RegName, is_Some (r2' !! x)) as Hr'_full_right;[intros x; destruct Hr'_full with x;eauto|].
+    pose proof (regmap_full_dom _ Hr'_full_left) as Hdom_r'.
+    pose proof (regmap_full_dom _ Hr'_full_right) as Hdom_s'.
+
+    iSplitR; [auto|]. rewrite /interp_conf.
+
+    iDestruct (na_inv_acc with "Hcls_inv HnaI") as ">(>(Hcls & Hcls' & Hscls & Hscls') & Hna & Hcls_close)";
+      [auto..|].
+
+    rewrite /registers_mapsto /spec_registers_mapsto.
+    rewrite -(insert_delete r1') -(insert_delete r2').
+
+    iDestruct (big_sepM_insert with "Hregs'") as "[HPC Hregs']". by apply lookup_delete.
+    destruct (Hr'_full_left r_t1) as [r1v ?].
+    iDestruct (big_sepM_delete _ _ r_t1 with "Hregs'") as "[Hr1 Hregs']".
+      by rewrite lookup_delete_ne //.
+    destruct (Hr'_full_left r_env) as [renvv ?].
+    iDestruct (big_sepM_delete _ _ r_env with "Hregs'") as "[Hrenv Hregs']".
+      by rewrite !lookup_delete_ne //.
+
+    iDestruct (big_sepM_insert with "Hsegs'") as "[HsPC Hsegs']". by apply lookup_delete.
+    destruct (Hr'_full_right r_t1) as [rs1v ?].
+    iDestruct (big_sepM_delete _ _ r_t1 with "Hsegs'") as "[Hs1 Hsegs']".
+      by rewrite lookup_delete_ne //.
+    destruct (Hr'_full_right r_env) as [senvv ?].
+    iDestruct (big_sepM_delete _ _ r_env with "Hsegs'") as "[Hsenv Hsegs']".
+      by rewrite !lookup_delete_ne //.
+
+    (* Run the closure activation code *)
+    iApply (closure_activation_spec with "[- $HPC $Hr1 $Hrenv $Hcls]");
+      [done| |done|..].
+    { intros ? [? ?]. constructor; try split; auto. }
+    rewrite updatePcPerm_cap_non_E //;[].
+    iIntros "(HPC & Hr1 & Hrenv & Hcls)".
+    iMod (closure_activation_spec_step with "[$Hspec $Hj $HsPC $Hs1 $Hsenv $Hscls]")
+      as "(Hj & HsPC & Hs1 & Hsenv & Hscls)";
+      [done| |done|auto..].
+    { intros ? [? ?]. constructor; try split; auto. }
+    rewrite updatePcPerm_cap_non_E //;[].
+
+    (* close the invariant for the closure *)
+    iDestruct ("Hcls_close" with "[Hcls Hcls' Hscls Hscls' $Hna]") as ">Hna".
+    { iNext. iFrame. }
+
+    destruct (Hr'_full_left r_t0) as [r0v Hr0v].
+    iDestruct (big_sepM_delete _ _ r_t0 with "Hregs'") as "[Hr0 Hregs']".
+      by rewrite !lookup_delete_ne // lookup_delete_ne //.
+
+   destruct (Hr'_full_right r_t0) as [s0v Hs0v].
+   iDestruct (big_sepM_delete _ _ r_t0 with "Hsegs'") as "[Hs0 Hsegs']".
+      by rewrite !lookup_delete_ne // lookup_delete_ne //.
+
+    iApply ((offset_incr_spec offset) with "[$Hspec $Hj $HPC $HsPC $Hr0 $Hs0 $Hrenv $Hsenv $Hregs' $Hsegs' $Hna $Hincr Hr1 Hs1 $Hcounter_inv]");
+      [| |apply Hcont_incr|apply Hcont_decr|auto|auto| | |apply Hnclose|..].
+    { eapply isCorrectPC_range_restrict; [apply Hvpc_counter|]. split;[clear;solve_addr|].
+      apply contiguous_between_bounds in Hcont_restc. apply Hcont_restc. }
+    { eapply isCorrectPC_range_restrict; [apply Hvspc_counter|]. split;[clear;solve_addr|].
+      apply contiguous_between_bounds in Hcont_srestc. apply Hcont_srestc. }
+    { rewrite !dom_delete_L Hdom_r'. clear. set_solver. }
+    { rewrite !dom_delete_L Hdom_s'. clear. set_solver. }
+    { iSplitL "Hr1";[eauto|]. iSplitL;[eauto|]. iSplit.
+      - unshelve iDestruct ("Hr'_valid" $! r_t0 _ _ _ Hr0v Hs0v) as "Hval";[auto|].
+        rewrite /interp//.
+      - iIntros (reg v1 v2 Hne Hv1s Hv2s).
+        destruct (decide (reg = r_t0));[subst;rewrite !lookup_delete in Hv1s Hv2s;done|rewrite !(lookup_delete_ne _ r_t0) // in Hv1s, Hv2s].
+        destruct (decide (reg = r_env));[subst;rewrite !lookup_delete in Hv1s Hv2s;done|rewrite !(lookup_delete_ne _ r_env)// in Hv1s Hv2s].
+        destruct (decide (reg = r_t1));[subst;rewrite !lookup_delete in Hv1s Hv2s;done|rewrite !(lookup_delete_ne _ r_t1)// in Hv1s Hv2s].
+        rewrite !(lookup_delete_ne _ PC)// in Hv1s Hv2s.
+       by unshelve iDestruct ("Hr'_valid" $! reg _ _ _ Hv1s Hv2s)  as "Hval";[done|]. }
+    { iNext. iIntros (?) "HH". iIntros (->). iApply "HH". eauto. }
+  Qed.
+
   Lemma read_read_neg_closure_valid read_prog read_neg_prog restc srestc
         read_readnegN countN count_clsN
         b_cls e_cls (* incr/decr closure *)
@@ -368,7 +523,118 @@ Section counter_example_preamble.
     { iNext. iIntros (?) "HH". iIntros (->). iApply "HH". eauto. }
   Qed.
 
+  Lemma read_offset_closure_valid read_prog read_offset_prog restc srestc
+        read_readnegN countN count_clsN
+        b_cls e_cls (* incr/decr closure *)
+        b_cls' e_cls' (* read/read_neg closure *)
+        pc_p pc_b pc_e counter_first counter_end linkc (* left PC values *)
+        pcs_p pcs_b pcs_e scounter_first scounter_end slinkc (* right PC values *)
+        b_cell e_cell (* left counter *)
+        bs_cell es_cell (* right counter *):
 
+    pc_p ≠ E → pcs_p ≠ E →
+
+    contiguous_between read_prog linkc counter_end →
+    contiguous_between read_offset_prog slinkc scounter_end →
+    isCorrectPC_range pc_p pc_b pc_e counter_first counter_end →
+    isCorrectPC_range pcs_p pcs_b pcs_e scounter_first scounter_end →
+
+    contiguous_between restc counter_first linkc →
+    contiguous_between srestc scounter_first slinkc →
+
+    (b_cell + 1)%a = Some e_cell →
+    (bs_cell + 1)%a = Some es_cell →
+    nclose specN ## ↑countN →
+
+    ⊢ (spec_ctx -∗ inv countN (offset_counter_inv offset b_cell bs_cell) -∗
+     na_inv logrel_nais read_readnegN (read_left read_prog ∗ offset_read_right offset read_offset_prog) -∗
+     na_inv logrel_nais count_clsN (cls_inv b_cls e_cls b_cls' e_cls' (WCap pc_p pc_b pc_e counter_first)
+                                            (WCap pc_p pc_b pc_e linkc) (WCap RWX b_cell e_cell b_cell)
+
+                                            (WCap pcs_p pcs_b pcs_e scounter_first) (WCap pcs_p pcs_b pcs_e slinkc)
+                                            (WCap RWX bs_cell es_cell bs_cell)) -∗
+     na_own logrel_nais ⊤ -∗
+    interp (WCap E b_cls' e_cls' b_cls',WCap E b_cls' e_cls' b_cls'))%I.
+  Proof.
+    iIntros (Hnp Hnps Hcont_incr Hcont_decr Hvpc_counter Hvspc_counter Hcont_restc Hcont_srestc Hbe_cell Hbes_cell Hnclose)
+            "#Hspec #Hcounter_inv #Hincr #Hcls_inv HnaI".
+    rewrite /interp fixpoint_interp1_eq /=. iSplit;auto.
+    iIntros (r') "". iNext. iModIntro.
+    iIntros "(#Hr_valid & Hregs' & Hsegs' & HnaI & Hj)". destruct r' as [r1' r2']. simpl.
+    iDestruct (interp_reg_eq _ _ (WCap RX b_cls e_cls b_cls) with "Hr_valid") as %Heq.
+    iDestruct "Hr_valid" as "[Hr'_full Hr'_valid]"; iDestruct "Hr'_full" as %Hr'_full.
+    assert (∀ x : RegName, is_Some (r1' !! x)) as Hr'_full_left;[intros x; destruct Hr'_full with x;eauto|].
+    assert (∀ x : RegName, is_Some (r2' !! x)) as Hr'_full_right;[intros x; destruct Hr'_full with x;eauto|].
+    pose proof (regmap_full_dom _ Hr'_full_left) as Hdom_r'.
+    pose proof (regmap_full_dom _ Hr'_full_right) as Hdom_s'.
+
+    iSplitR; [auto|]. rewrite /interp_conf.
+
+    iDestruct (na_inv_acc with "Hcls_inv HnaI") as ">(>(Hcls & Hcls' & Hscls & Hscls') & Hna & Hcls_close)";
+      [auto..|].
+
+    rewrite /registers_mapsto /spec_registers_mapsto.
+    rewrite -(insert_delete r1') -(insert_delete r2').
+
+    iDestruct (big_sepM_insert with "Hregs'") as "[HPC Hregs']". by apply lookup_delete.
+    destruct (Hr'_full_left r_t1) as [r1v ?].
+    iDestruct (big_sepM_delete _ _ r_t1 with "Hregs'") as "[Hr1 Hregs']".
+      by rewrite lookup_delete_ne //.
+    destruct (Hr'_full_left r_env) as [renvv ?].
+    iDestruct (big_sepM_delete _ _ r_env with "Hregs'") as "[Hrenv Hregs']".
+      by rewrite !lookup_delete_ne //.
+
+    iDestruct (big_sepM_insert with "Hsegs'") as "[HsPC Hsegs']". by apply lookup_delete.
+    destruct (Hr'_full_right r_t1) as [rs1v ?].
+    iDestruct (big_sepM_delete _ _ r_t1 with "Hsegs'") as "[Hs1 Hsegs']".
+      by rewrite lookup_delete_ne //.
+    destruct (Hr'_full_right r_env) as [senvv ?].
+    iDestruct (big_sepM_delete _ _ r_env with "Hsegs'") as "[Hsenv Hsegs']".
+      by rewrite !lookup_delete_ne //.
+
+    (* Run the closure activation code *)
+    iApply (closure_activation_spec with "[- $HPC $Hr1 $Hrenv $Hcls']");
+      [done| |done|..].
+    { intros ? [? ?]. constructor; try split; auto. }
+    rewrite updatePcPerm_cap_non_E //;[].
+    iIntros "(HPC & Hr1 & Hrenv & Hcls')".
+    iMod (closure_activation_spec_step with "[$Hspec $Hj $HsPC $Hs1 $Hsenv $Hscls']")
+      as "(Hj & HsPC & Hs1 & Hsenv & Hscls')";
+      [done| |done|auto..].
+    { intros ? [? ?]. constructor; try split; auto. }
+    rewrite updatePcPerm_cap_non_E //;[].
+
+    (* close the invariant for the closure *)
+    iDestruct ("Hcls_close" with "[Hcls Hcls' Hscls Hscls' $Hna]") as ">Hna".
+    { iNext. iFrame. }
+
+    destruct (Hr'_full_left r_t0) as [r0v Hr0v].
+    iDestruct (big_sepM_delete _ _ r_t0 with "Hregs'") as "[Hr0 Hregs']".
+      by rewrite !lookup_delete_ne // lookup_delete_ne //.
+
+   destruct (Hr'_full_right r_t0) as [s0v Hs0v].
+   iDestruct (big_sepM_delete _ _ r_t0 with "Hsegs'") as "[Hs0 Hsegs']".
+     by rewrite !lookup_delete_ne // lookup_delete_ne //.
+
+   iApply (offset_read_spec with "[$Hspec $Hj $HPC $HsPC $Hr0 $Hs0 $Hrenv $Hsenv $Hregs' $Hsegs' $Hna $Hincr Hr1 Hs1 $Hcounter_inv]");
+      [| |apply Hcont_incr|apply Hcont_decr|auto|auto| | |apply Hnclose|..].
+    { eapply isCorrectPC_range_restrict; [apply Hvpc_counter|]. split;[|clear;solve_addr].
+      apply contiguous_between_bounds in Hcont_restc. apply Hcont_restc. }
+    { eapply isCorrectPC_range_restrict; [apply Hvspc_counter|]. split;[|clear;solve_addr].
+      apply contiguous_between_bounds in Hcont_srestc. apply Hcont_srestc. }
+    { rewrite !dom_delete_L Hdom_r'. clear. set_solver. }
+    { rewrite !dom_delete_L Hdom_s'. clear. set_solver. }
+    { iSplitL "Hr1";[eauto|]. iSplitL;[eauto|]. iSplit.
+      - unshelve iDestruct ("Hr'_valid" $! r_t0 _ _ _ Hr0v Hs0v) as "Hval";[auto|]. rewrite /interp//.
+      - iIntros (reg v1 v2 Hne Hv1s Hv2s).
+            destruct (decide (reg = r_t0));[subst;rewrite !lookup_delete in Hv1s Hv2s;done|rewrite !(lookup_delete_ne _ r_t0) // in Hv1s, Hv2s].
+            destruct (decide (reg = r_env));[subst;rewrite !lookup_delete in Hv1s Hv2s;done|rewrite !(lookup_delete_ne _ r_env)// in Hv1s Hv2s].
+            destruct (decide (reg = r_t1));[subst;rewrite !lookup_delete in Hv1s Hv2s;done|rewrite !(lookup_delete_ne _ r_t1)// in Hv1s Hv2s].
+            rewrite !(lookup_delete_ne _ PC)// in Hv1s Hv2s.
+              by unshelve iDestruct ("Hr'_valid" $! reg _ _ _ Hv1s Hv2s)  as "Hval";[done|].
+    }
+    { iNext. iIntros (?) "HH". iIntros (->). iApply "HH". eauto. }
+  Qed.
 
 
   Definition countN : namespace := nroot .@ "awkN".
@@ -979,5 +1245,605 @@ Section counter_example_preamble.
     iExists r0. iFrame.
   Qed.
 
+  Lemma offset_counter_preamble_spec (f_m offset_to_counter: Z) r
+        pc_p pc_b pc_e pcs_p pcs_b pcs_e
+        ai a_first a_end b_link e_link a_link a_entry
+        ais s_first s_end bs_link es_link s_link s_entry
+        mallocN b_m e_m
+        ai_counter counter_first counter_end a_move
+        ais_counter counter_sfirst counter_send s_move :
+
+    isCorrectPC_range pc_p pc_b pc_e a_first a_end →
+    isCorrectPC_range pcs_p pcs_b pcs_e s_first s_end →
+
+    contiguous_between ai a_first a_end →
+    contiguous_between ais s_first s_end →
+
+
+    withinBounds b_link e_link a_entry = true →
+    (a_link + f_m)%a = Some a_entry →
+
+    withinBounds bs_link es_link s_entry = true →
+    (s_link + f_m)%a = Some s_entry →
+
+
+    (a_first + counter_preamble_move_offset)%a = Some a_move →
+    (a_move + offset_to_counter)%a = Some counter_first →
+    isCorrectPC_range pc_p pc_b pc_e counter_first counter_end →
+    contiguous_between ai_counter counter_first counter_end →
+
+    (s_first + counter_preamble_move_offset)%a = Some s_move →
+    (s_move + offset_to_counter)%a = Some counter_sfirst →
+    isCorrectPC_range pcs_p pcs_b pcs_e counter_sfirst counter_send →
+    contiguous_between ais_counter counter_sfirst counter_send →
+
+    spec_ctx
+    (* Code of the preambles *)
+    ∗ counter_left_preamble f_m offset_to_counter ai
+    ∗ counter_offset_preamble f_m offset_to_counter ais
+
+    (* Code of the counter examples themselves *)
+    ∗ counter_left ai_counter
+    ∗ counter_offset ais_counter
+
+    (** Resources for malloc and assert **)
+    (* assume that a pointer to the linking table (where the malloc capa is) is at offset 0 of PC *)
+    ∗ na_inv logrel_nais mallocN (malloc_inv_binary b_m e_m)
+    ∗ pc_b ↦ₐ (WCap RO b_link e_link a_link)
+    ∗ a_entry ↦ₐ (WCap E b_m e_m b_m)
+    ∗ pcs_b ↣ₐ (WCap RO bs_link es_link s_link)
+    ∗ s_entry ↣ₐ (WCap E b_m e_m b_m)
+
+    -∗
+    interp_expr interp r (WCap pc_p pc_b pc_e a_first,WCap pcs_p pcs_b pcs_e s_first).
+  Proof.
+    rewrite /interp_expr /=.
+    iIntros (Hvpc Hvpc' Hcont Hcont' Hwb_malloc Ha_entry Hwb_malloc' Hs_entry
+                  Ha_lea H_counter_offset Hvpc_counter Hcont_counter
+                  Ha_lea' H_counter_offset' Hvpc_counter'). iIntros (Hcont_counter').
+    iIntros "(#Hspec & Hprog & Hsprog & Hcounter & Hscounter & #Hinv_malloc & Hpc_b & Ha_entry & Hpcs_b & Hs_entry)
+             ([#Hr_full #Hr_valid] & Hregs & Hsegs & HnaI & Hj)".
+    iDestruct "Hr_full" as %Hr_full.
+    rewrite /full_map.
+    iSplitR; auto. rewrite /interp_conf.
+
+    (* put the code for the counter example in an invariant *)
+    (* we separate the invariants into its tree functions *)
+    iDestruct (contiguous_between_program_split with "Hcounter") as (incr_prog restc linkc)
+                                                                   "(Hincr & Hread & #Hcont)";[apply Hcont_counter|].
+    iDestruct "Hcont" as %(Hcont_incr & Hcont_restc & Heqappc & Hlinkrestc).
+    iDestruct (contiguous_between_program_split with "Hscounter") as (decr_prog restc' linkc')
+                                                                   "(Hdecr & Hreadneg & #Hcont)";[apply Hcont_counter'|].
+    iDestruct "Hcont" as %(Hcont_decr & Hcont_restc' & Heqappc' & Hlinkrestc').
+    iDestruct (big_sepL2_length with "Hincr") as %incr_length.
+    iDestruct (big_sepL2_length with "Hread") as %read_length.
+    iDestruct (big_sepL2_length with "Hdecr") as %decr_length.
+    iDestruct (big_sepL2_length with "Hreadneg") as %readneg_length.
+
+    iCombine "Hincr" "Hdecr" as "Hincr".
+    iCombine "Hread" "Hreadneg" as "Hread".
+
+    iDestruct (na_inv_alloc logrel_nais _ count_incrN with "Hincr") as ">#Hincr".
+    iDestruct (na_inv_alloc logrel_nais _ count_readN with "Hread") as ">#Hread".
+
+    rewrite /registers_mapsto /spec_registers_mapsto.
+    iDestruct (big_sepM_delete _ _ PC with "Hregs") as "[HPC Hregs]".
+      by rewrite lookup_insert //. rewrite delete_insert_delete //.
+    iDestruct (big_sepM_delete _ _ PC with "Hsegs") as "[HsPC Hsegs]".
+      by rewrite lookup_insert //. rewrite delete_insert_delete //.
+    destruct (Hr_full r_t0) as [ [r0 Hr0] [s0 Hs0] ].
+    iDestruct (big_sepM_delete _ _ r_t0 with "Hregs") as "[Hr0 Hregs]". by rewrite !lookup_delete_ne//.
+    iDestruct (big_sepM_delete _ _ r_t0 with "Hsegs") as "[Hs0 Hsegs]". by rewrite !lookup_delete_ne//.
+    assert (∀ x : RegName, is_Some (r.1 !! x)) as Hr'_full_left;[intros x; destruct Hr_full with x;eauto|].
+    assert (∀ x : RegName, is_Some (r.2 !! x)) as Hr'_full_right;[intros x; destruct Hr_full with x;eauto|].
+    pose proof (regmap_full_dom _ Hr'_full_left) as Hdom_r'.
+    pose proof (regmap_full_dom _ Hr'_full_right) as Hdom_s'.
+
+    iDestruct (big_sepL2_length with "Hprog") as %Hlength.
+    iDestruct (big_sepL2_length with "Hsprog") as %Hslength.
+
+    assert (pc_p ≠ E).
+    { eapply isCorrectPC_range_perm_non_E. eapply Hvpc.
+      pose proof (contiguous_between_length _ _ _ Hcont) as HH. rewrite Hlength /= in HH.
+      revert HH; clear; solve_addr. }
+
+    assert (pcs_p ≠ E).
+    { eapply isCorrectPC_range_perm_non_E. eapply Hvpc'.
+      pose proof (contiguous_between_length _ _ _ Hcont') as HH. rewrite Hslength /= in HH.
+      revert HH; clear; solve_addr. }
+
+    (* malloc 1 *)
+    iDestruct (contiguous_between_program_split with "Hprog") as
+        (ai_malloc ai_rest a_malloc_end) "(Hmalloc & Hprog & #Hcont)"; [apply Hcont|].
+    iDestruct "Hcont" as %(Hcont_malloc & Hcont_rest & Heqapp & Hlink).
+    iDestruct (contiguous_between_program_split with "Hsprog") as
+        (ais_malloc ais_rest as_malloc_end) "(Hsmalloc & Hsprog & #Hcont)"; [apply Hcont'|].
+    iDestruct "Hcont" as %(Hcont_smalloc & Hcont_srest & Heqapp' & Hlink').
+
+    iDestruct (big_sepL2_length with "Hmalloc") as %Hai_malloc_len.
+    iDestruct (big_sepL2_length with "Hsmalloc") as %Hais_malloc_len.
+
+    assert (isCorrectPC_range pc_p pc_b pc_e a_first a_malloc_end) as Hvpc1.
+    { eapply isCorrectPC_range_restrict. apply Hvpc.
+      generalize (contiguous_between_bounds _ _ _ Hcont_rest). clear; solve_addr. }
+    assert (isCorrectPC_range pc_p pc_b pc_e a_malloc_end a_end) as Hvpc2.
+    { eapply isCorrectPC_range_restrict. apply Hvpc.
+      generalize (contiguous_between_bounds _ _ _ Hcont_malloc). clear; solve_addr. }
+    assert (isCorrectPC_range pcs_p pcs_b pcs_e s_first as_malloc_end) as Hvpc1'.
+    { eapply isCorrectPC_range_restrict. apply Hvpc'.
+      generalize (contiguous_between_bounds _ _ _ Hcont_srest). clear; solve_addr. }
+    assert (isCorrectPC_range pcs_p pcs_b pcs_e as_malloc_end s_end) as Hvpc2'.
+    { eapply isCorrectPC_range_restrict. apply Hvpc'.
+      generalize (contiguous_between_bounds _ _ _ Hcont_smalloc). clear; solve_addr. }
+
+    rewrite - !/(malloc _ _ _).
+    iApply (wp_wand with "[-]").
+    iApply (malloc_s_spec with "[- $Hspec $Hj $HPC $HsPC $Hmalloc $Hsmalloc $Hpc_b $Hpcs_b $Ha_entry $Hs_entry $Hr0 $Hs0 $Hregs $Hsegs $Hinv_malloc $HnaI]");
+      [apply Hvpc1|apply Hvpc1'|eapply Hcont_malloc|eapply Hcont_smalloc|eapply Hwb_malloc|eapply Ha_entry|eapply Hwb_malloc'|eapply Hs_entry|auto..].
+    { rewrite !dom_delete_L Hdom_r' difference_difference_L //. }
+    { rewrite !dom_delete_L Hdom_s' difference_difference_L //. }
+    iNext. iIntros "(Hj & HPC & HsPC & Hmalloc & Hsmalloc & Hpc_b & Hpcs_b & Ha_entry & Hs_entry & HH & Hr0 & Hs0 & HnaI & Hregs & Hsegs)".
+    iDestruct "HH" as (b_cell e_cell Hbe_cell) "(Hr1 & Hs1 & Hcell & Hscell)".
+    iDestruct (region_mapsto_single with "Hcell") as (cellv) "(Hcell & _)". revert Hbe_cell; clear; solve_addr.
+    iDestruct (region_mapsto_single_spec with "Hscell") as (cellv') "(Hscell & _)". revert Hbe_cell; clear; solve_addr.
+    iDestruct (big_sepL2_length with "Hprog") as %Hlength_rest.
+    iDestruct (big_sepL2_length with "Hsprog") as %Hlength_srest.
+    2: { iIntros (?) "[HH | ->]". iApply "HH". iIntros (Hv). inversion Hv. }
+
+    destruct ai_rest as [| a l]; [by inversion Hlength|].
+    destruct ais_rest as [| a' l']; [by inversion Hslength|].
+    pose proof (contiguous_between_cons_inv_first _ _ _ _ Hcont_rest) as ->.
+    pose proof (contiguous_between_cons_inv_first _ _ _ _ Hcont_srest) as ->.
+    (* store_z r_t1 0 *)
+    destruct l as [| ? l]; [by inversion Hlength_rest|].
+    destruct l' as [| ? l']; [by inversion Hlength_srest|].
+    iPrologue_both "Hprog" "Hsprog".
+    iMod (step_store_success_z _ [SeqCtx] with "[$Hspec $Hj $HsPC $Hs1 $Hsi $Hscell]")
+      as "(Hj & HsPC & Hsprog_done & Hs1 & Hb_scell)";
+      [apply decode_encode_instrW_inv|iCorrectPC as_malloc_end s_end|
+       iContiguous_next Hcont_srest 0|auto..].
+    { split; auto. apply le_addr_withinBounds; revert Hbe_cell; clear; solve_addr. }
+    iApply (wp_store_success_z with "[$HPC $Hr1 $Hi $Hcell]");
+      [apply decode_encode_instrW_inv|iCorrectPC a_malloc_end a_end|
+       iContiguous_next Hcont_rest 0|..].
+    { auto. }
+    { apply le_addr_withinBounds; revert Hbe_cell; clear; solve_addr. }
+    iEpilogue_both "(HPC & Hprog_done & Hr1 & Hb_cell)".
+    iCombine "Hprog_done" "Hmalloc" as "Hprog_done". iCombine "Hsprog_done" "Hsmalloc" as "Hsprog_done".
+    (* move_r r_t2 r_t1 *)
+    iDestruct (big_sepM_delete _ _ r_t2 with "Hregs") as "[Hr2 Hregs]".
+      by rewrite lookup_insert. rewrite delete_insert_delete.
+    iDestruct (big_sepM_delete _ _ r_t2 with "Hsegs") as "[Hs2 Hsegs]".
+      by rewrite lookup_insert. rewrite delete_insert_delete.
+    destruct l as [| a_move' l]; [by inversion Hlength_rest|]. destruct l' as [| as_move' l']; [by inversion Hlength_srest|].
+    iPrologue_both "Hprog" "Hsprog".
+    iMod (step_move_success_reg _ [SeqCtx] _ _ _ _ _ _ r_t2 _ r_t1 with "[$Hspec $Hj $HsPC $Hsi $Hs1 $Hs2]")
+      as "(Hj & HsPC & Hsi & Hs2 & Hs1)";
+      [eapply decode_encode_instrW_inv|iCorrectPC as_malloc_end s_end|iContiguous_next Hcont_srest 1|auto..].
+    iApply (wp_move_success_reg _ _ _ _ _ _ _ r_t2 _ r_t1 with "[$HPC $Hi $Hr1 $Hr2]");
+      [eapply decode_encode_instrW_inv|iCorrectPC a_malloc_end a_end|iContiguous_next Hcont_rest 1|..].
+    iEpilogue_both "(HPC & Hi & Hr2 & Hr1)". iCombinePtrn.
+    (* move_r r_t1 PC *)
+    destruct l as [| ? l]; [by inversion Hlength_rest|]. destruct l' as [| ? l']; [by inversion Hlength_srest|].
+    iPrologue_both "Hprog" "Hsprog".
+    iMod (step_move_success_reg_fromPC _ [SeqCtx] with "[$Hspec $Hj $HsPC $Hsi $Hs1]")
+      as "(Hj & HsPC & Hsi & Hs1)";
+      [eapply decode_encode_instrW_inv|iCorrectPC as_malloc_end s_end|iContiguous_next Hcont_srest 2|auto..].
+    iApply (wp_move_success_reg_fromPC with "[$HPC $Hi $Hr1]");
+      [eapply decode_encode_instrW_inv|iCorrectPC a_malloc_end a_end|iContiguous_next Hcont_rest 2|..].
+    iEpilogue_both "(HPC & Hi & Hr1)". iCombinePtrn.
+    (* move_r r_t8 r_t2 *)
+    destruct Hr_full with r_t8 as [ [? Hrt8] [? Hst8] ].
+    iDestruct (big_sepM_delete _ _ r_t8 with "Hregs") as "[Hr_t8 Hregs]".
+    { rewrite lookup_delete_ne;[|by auto]. rewrite !lookup_insert_ne;auto; rewrite !lookup_delete_ne;auto. eauto. }
+    iDestruct (big_sepM_delete _ _ r_t8 with "Hsegs") as "[Hr_s8 Hsegs]".
+    { rewrite lookup_delete_ne;[|by auto]. rewrite !lookup_insert_ne;auto; rewrite !lookup_delete_ne;auto. eauto. }
+    destruct l as [| ? l]; [by inversion Hlength_rest|]. destruct l' as [| ? l']; [by inversion Hlength_srest|].
+    iPrologue_both "Hprog" "Hsprog".
+    iMod (step_move_success_reg _ [SeqCtx] with "[$Hspec $Hj $HsPC $Hsi $Hr_s8 $Hs2]")
+      as "(Hj & HsPC & Hsi & Hs_t8 & Hs2)";
+      [eapply decode_encode_instrW_inv|iCorrectPC as_malloc_end s_end|iContiguous_next Hcont_srest 3|auto..].
+    iApply (wp_move_success_reg with "[$HPC $Hi $Hr_t8 $Hr2]");
+      [eapply decode_encode_instrW_inv|iCorrectPC a_malloc_end a_end|iContiguous_next Hcont_rest 3|..].
+    iEpilogue_both "(HPC & Hi & Hr_t8 & Hr2)". iCombinePtrn.
+    iDestruct (big_sepM_insert _ _ r_t8 with "[$Hregs $Hr_t8]") as "Hregs";[apply lookup_delete|rewrite insert_delete].
+    iDestruct (big_sepM_insert _ _ r_t8 with "[$Hsegs $Hs_t8]") as "Hsegs";[apply lookup_delete|rewrite insert_delete].
+    (* move_r r_t9 r_t1 *)
+    destruct Hr_full with r_t9 as [ [? Hrt9] [? Hst9] ].
+    iDestruct (big_sepM_delete _ _ r_t9 with "Hregs") as "[Hr_t8 Hregs]".
+    { rewrite lookup_insert_ne;[|by auto]. rewrite lookup_delete_ne;auto. rewrite !lookup_insert_ne;auto; rewrite !lookup_delete_ne;auto. eauto. }
+    iDestruct (big_sepM_delete _ _ r_t9 with "Hsegs") as "[Hs_t8 Hsegs]".
+    { rewrite lookup_insert_ne;[|by auto]. rewrite lookup_delete_ne;auto. rewrite !lookup_insert_ne;auto; rewrite !lookup_delete_ne;auto. eauto. }
+    destruct l as [| ? l]; [by inversion Hlength_rest|]. destruct l' as [| ? l']; [by inversion Hlength_srest|].
+    iPrologue_both "Hprog" "Hsprog".
+    iMod (step_move_success_reg _ [SeqCtx] with "[$Hspec $Hj $HsPC $Hsi $Hs_t8 $Hs1]")
+      as "(Hj & HsPC & Hsi & Hs_t8 & Hs1)";
+      [eapply decode_encode_instrW_inv|iCorrectPC as_malloc_end s_end|iContiguous_next Hcont_srest 4|auto..].
+    iApply (wp_move_success_reg with "[$HPC $Hi $Hr_t8 $Hr1]");
+      [eapply decode_encode_instrW_inv|iCorrectPC a_malloc_end a_end|iContiguous_next Hcont_rest 4|..].
+    iEpilogue_both "(HPC & Hi & Hr_t8 & Hr1)". iCombinePtrn.
+    iDestruct (big_sepM_insert _ _ r_t9 with "[$Hregs $Hr_t8]") as "Hregs";[apply lookup_delete|rewrite insert_delete].
+    iDestruct (big_sepM_insert _ _ r_t9 with "[$Hsegs $Hs_t8]") as "Hsegs";[apply lookup_delete|rewrite insert_delete].
+
+    (* lea_z r_t1 offset_to_awkward *)
+
+    assert (a_move' = a_move) as ->.
+    { assert ((a_first + (length ai_malloc + 2))%a = Some a_move') as HH.
+      { rewrite Hai_malloc_len /= in Hlink |- *.
+        generalize (contiguous_between_incr_addr_middle _ _ _ 0 2 _ _ Hcont_rest eq_refl eq_refl).
+        revert Hlink; clear; solve_addr. }
+      revert HH Ha_lea. rewrite Hai_malloc_len. cbn. clear.
+      unfold counter_preamble_move_offset. solve_addr. }
+    assert (as_move' = s_move) as ->.
+    { assert ((s_first + (length ais_malloc + 2))%a = Some as_move') as HH.
+      { rewrite Hais_malloc_len /= in Hlink' |- *.
+        generalize (contiguous_between_incr_addr_middle _ _ _ 0 2 _ _ Hcont_srest eq_refl eq_refl).
+        revert Hlink'; clear; solve_addr. }
+      revert HH Ha_lea'. rewrite Hais_malloc_len. cbn. clear.
+      unfold counter_preamble_move_offset. solve_addr. }
+
+    destruct l as [| ? l]; [by inversion Hlength_rest|]. destruct l' as [| ? l']; [by inversion Hlength_srest|].
+    iPrologue_both "Hprog" "Hsprog".
+    iMod (step_lea_success_z _ [SeqCtx] _ _ _ _ _ _ _ _ _ _ _ _ counter_sfirst with "[$Hspec $Hj $HsPC $Hsi $Hs1]")
+      as "(Hj & HsPC & Hsi & Hs1)";
+      [eapply decode_encode_instrW_inv|iCorrectPC as_malloc_end s_end|iContiguous_next Hcont_srest 5
+       |assumption|done|auto..].
+    iApply (wp_lea_success_z _ _ _ _ _ _ _ _ _ _ _ _ _ counter_first with "[$HPC $Hi $Hr1]");
+      [eapply decode_encode_instrW_inv|iCorrectPC a_malloc_end a_end|iContiguous_next Hcont_rest 5
+       |assumption|done|..].
+    (* { destruct (isCorrectPC_range_perm _ _ _ _ _ _ Hvpc) as [-> | [-> | ->] ]; auto. *)
+    (*   generalize (contiguous_between_middle_bounds _ (length ai_malloc) a_malloc_end _ _ Hcont ltac:(subst ai; rewrite list_lookup_middle; auto)). clear. solve_addr. } *)
+    iEpilogue_both "(HPC & Hi & Hr1)". iCombinePtrn.
+    (* crtcls *)
+
+    iDestruct (contiguous_between_program_split with "Hprog") as
+        (ai_crtcls ai_rest a_crtcls_end) "(Hcrtcls & Hprog & #Hcont)".
+    { epose proof (contiguous_between_incr_addr _ 6%nat _ _ _ Hcont_rest eq_refl).
+      eapply contiguous_between_app with (a1:=[_;_;_;_;_;_]). 2: eapply Hcont_rest.
+      all: eauto. }
+    iDestruct "Hcont" as %(Hcont_crtcls & Hcont_rest1 & Heqapp1 & Hlink1).
+    iDestruct (contiguous_between_program_split with "Hsprog") as
+        (ais_crtcls ais_rest as_crtcls_end) "(Hscrtcls & Hsprog & #Hcont)".
+    { epose proof (contiguous_between_incr_addr _ 6%nat _ _ _ Hcont_srest eq_refl).
+      eapply contiguous_between_app with (a1:=[_;_;_;_;_;_]). 2: eapply Hcont_srest.
+      all: eauto. }
+    iDestruct "Hcont" as %(Hcont_scrtcls & Hcont_rest1' & Heqapp1' & Hlink1').
+
+    assert (a_malloc_end <= f7)%a as Ha1_after_malloc.
+    { eapply contiguous_between_middle_bounds'. apply Hcont_rest. repeat constructor. }
+    assert (as_malloc_end <= f8)%a as Ha1_after_malloc'.
+    { eapply contiguous_between_middle_bounds'. apply Hcont_srest. repeat constructor. }
+
+    iApply (wp_wand with "[-]").
+    iApply (crtcls_spec with "[- $Hspec $Hj $HPC $HsPC $Hcrtcls $Hscrtcls $Hpc_b $Hpcs_b $Ha_entry $Hs_entry $Hr0 $Hs0 $Hregs $Hsegs $Hr1 $Hs1 $Hr2 $Hs2 $HnaI $Hinv_malloc]");
+      [| |apply Hcont_crtcls|apply Hcont_scrtcls|apply Hwb_malloc|apply Ha_entry|apply Hwb_malloc'|apply Hs_entry| | |done|auto|..].
+    { eapply isCorrectPC_range_restrict. apply Hvpc2. split; auto.
+      eapply contiguous_between_bounds. apply Hcont_rest1. }
+    { eapply isCorrectPC_range_restrict. apply Hvpc2'. split; auto.
+      eapply contiguous_between_bounds. apply Hcont_rest1'. }
+    { rewrite !dom_insert_L dom_delete_L !dom_insert_L !dom_delete_L Hdom_r'.
+      clear. set_solver-. }
+    { rewrite !dom_insert_L dom_delete_L !dom_insert_L !dom_delete_L Hdom_s'.
+      clear. set_solver-. }
+    2: { iIntros (?) "[ H | -> ]". iApply "H". iIntros (HC). congruence. }
+    iNext. iIntros "(Hj & HPC & Hcrtcls & HsPC & Hscrtcls & Hpc_b & Hpcs_b & Ha_entry & Hs_entry & HH)".
+    iDestruct "HH" as (b_cls e_cls Hbe_cls) "(Hr1 & Hs1 & Hbe_cls & Hbes_cls & Hr0 & Hs0 & Hr2 & Hs2 & HnaI & Hregs & Hsegs)".
+    iDestruct (big_sepL2_length with "Hprog") as %Hlength_rest1.
+    iDestruct (big_sepL2_length with "Hsprog") as %Hlength_rest1'.
+
+    (* register map cleanup *)
+
+    assert (forall (r : gmap RegName Word) w1 w2, <[r_t3:=WInt 0%Z]> (<[r_t4:=WInt 0%Z]> (<[r_t5:=WInt 0%Z]> (<[r_t6:=WInt 0%Z]> (<[r_t7:=WInt 0%Z]>
+                  (<[r_t9:=w1]> (<[r_t8:=w2]>
+                  (delete r_t2 (<[r_t3:=WInt 0%Z]> (<[r_t4:=WInt 0%Z]> (<[r_t5:=WInt 0%Z]> (delete r_t1 (delete r_t0 (delete PC r))))))))))))) =
+                 <[r_t9:=w1]> (<[r_t8:=w2]> (<[r_t3:=WInt 0%Z]> (<[r_t4:=WInt 0%Z]>
+                  (<[r_t5:=WInt 0%Z]> (<[r_t6:=WInt 0%Z]> (<[r_t7:=WInt 0%Z]> (delete r_t2 (delete r_t1 (delete r_t0 (delete PC r))))))))))
+           ) as Heqregs1.
+    { clear. intros r w1 w2. set (regs := <[r_t9:=w1]> (<[r_t8:=w2]>
+                                     (<[r_t3:=WInt 0%Z]> (<[r_t4:=WInt 0%Z]> (<[r_t5:=WInt 0%Z]> (<[r_t6:=WInt 0%Z]> (<[r_t7:=WInt 0%Z]>
+                                       (delete r_t2 (delete r_t1 (delete r_t0 (delete PC r))))))))))).
+      rewrite !delete_insert_ne;auto.
+      repeat (rewrite (insert_commute _ r_t3);[|by auto]). rewrite insert_insert.
+      repeat (rewrite (insert_commute _ r_t4);[|by auto]). rewrite insert_insert.
+      repeat (rewrite (insert_commute _ r_t5);[|by auto]). rewrite insert_insert.
+      repeat (rewrite (insert_commute _ r_t6);[|by auto]). repeat (rewrite (insert_commute _ r_t7);[|by auto]).
+      auto.
+    }
+
+    rewrite (Heqregs1 r.1). rewrite (Heqregs1 r.2).
+
+    assert (isCorrectPC_range pc_p pc_b pc_e a_crtcls_end a_end) as Hvpc3.
+    { eapply isCorrectPC_range_restrict. apply Hvpc2.
+      generalize (contiguous_between_bounds _ _ _ Hcont_rest1).
+      revert Ha1_after_malloc Hlink1. clear; solve_addr. }
+    assert (isCorrectPC_range pcs_p pcs_b pcs_e as_crtcls_end s_end) as Hvpc3'.
+    { eapply isCorrectPC_range_restrict. apply Hvpc2'.
+      generalize (contiguous_between_bounds _ _ _ Hcont_rest1').
+      revert Ha1_after_malloc' Hlink1'. clear; solve_addr. }
+
+    (* move r_t10 r_t1 *)
+    destruct Hr_full with r_t10 as [ [? Hrt10] [? Hst10] ].
+    iDestruct (big_sepM_delete _ _ r_t10 with "Hregs") as "[Hr_t10 Hregs]".
+    { rewrite !lookup_insert_ne;auto. rewrite !lookup_delete_ne;auto. eauto. }
+    iDestruct (big_sepM_delete _ _ r_t10 with "Hsegs") as "[Hs_t10 Hsegs]".
+    { rewrite !lookup_insert_ne;auto. rewrite !lookup_delete_ne;auto. eauto. }
+
+    destruct ai_rest as [| ? ai_rest]; [by inversion Hlength_rest1|].
+    destruct ais_rest as [| ? ais_rest]; [by inversion Hlength_rest1'|].
+    pose proof (contiguous_between_cons_inv_first _ _ _ _ Hcont_rest1) as ->.
+    pose proof (contiguous_between_cons_inv_first _ _ _ _ Hcont_rest1') as ->.
+    destruct ai_rest as [| ? ai_rest]; [by inversion Hlength_rest1|].
+    destruct ais_rest as [| ? ais_rest]; [by inversion Hlength_rest1'|].
+
+    iPrologue_both "Hprog" "Hsprog".
+    iMod (step_move_success_reg _ [SeqCtx] with "[$Hspec $Hj $HsPC $Hsi $Hs_t10 $Hs1]")
+      as "(Hj & HsPC & Hsi & Hs_t10 & Hs1)";
+      [eapply decode_encode_instrW_inv|iCorrectPC as_crtcls_end s_end|iContiguous_next Hcont_rest1' 0|auto..].
+    iApply (wp_move_success_reg with "[$HPC $Hi $Hr_t10 $Hr1]");
+      [eapply decode_encode_instrW_inv|iCorrectPC a_crtcls_end a_end|iContiguous_next Hcont_rest1 0|..].
+    iEpilogue_both "(HPC & Hi & Hr_t10 & Hr1)". iCombinePtrn.
+    iDestruct (big_sepM_insert _ _ r_t10 with "[$Hregs $Hr_t10]") as "Hregs";[apply lookup_delete|rewrite insert_delete].
+    iDestruct (big_sepM_insert _ _ r_t10 with "[$Hsegs $Hs_t10]") as "Hsegs";[apply lookup_delete|rewrite insert_delete].
+    (* move r_t2 r_t8 *)
+    iDestruct (big_sepM_delete _ _ r_t8 with "Hregs") as "[Hr_t8 Hregs]".
+    { rewrite lookup_insert_ne// lookup_insert_ne// lookup_insert. eauto. }
+    iDestruct (big_sepM_delete _ _ r_t8 with "Hsegs") as "[Hs_t8 Hsegs]".
+    { rewrite lookup_insert_ne// lookup_insert_ne// lookup_insert. eauto. }
+    destruct ai_rest as [| ? ai_rest]; [by inversion Hlength_rest1|]. destruct ais_rest as [| ? ais_rest]; [by inversion Hlength_rest1'|].
+    iPrologue_both "Hprog" "Hsprog".
+    iMod (step_move_success_reg _ [SeqCtx] with "[$Hspec $Hj $HsPC $Hsi $Hs2 $Hs_t8]")
+      as "(Hj & HsPC & Hsi & Hs2 & Hs_t8)";
+      [eapply decode_encode_instrW_inv|iCorrectPC as_crtcls_end s_end|iContiguous_next Hcont_rest1' 1|auto..].
+    iApply (wp_move_success_reg with "[$HPC $Hi $Hr2 $Hr_t8]");
+      [eapply decode_encode_instrW_inv|iCorrectPC a_crtcls_end a_end|iContiguous_next Hcont_rest1 1|..].
+    iEpilogue_both "(HPC & Hi & Hr2 & Hr_t8)". iCombinePtrn.
+    iDestruct (big_sepM_insert _ _ r_t8 with "[$Hregs $Hr_t8]") as "Hregs";[apply lookup_delete|].
+    rewrite insert_delete (insert_commute _ r_t8 r_t10) // (insert_commute _ r_t8 r_t9)// insert_insert.
+    iDestruct (big_sepM_insert _ _ r_t8 with "[$Hsegs $Hs_t8]") as "Hsegs";[apply lookup_delete|].
+    rewrite insert_delete (insert_commute _ r_t8 r_t10)// (insert_commute _ r_t8 r_t9)// insert_insert.
+    (* move r_t1 r_t9 *)
+    iDestruct (big_sepM_delete _ _ r_t9 with "Hregs") as "[Hr_t9 Hregs]";[rewrite lookup_insert_ne// lookup_insert;eauto|].
+    iDestruct (big_sepM_delete _ _ r_t9 with "Hsegs") as "[Hs_t9 Hsegs]";[rewrite lookup_insert_ne// lookup_insert;eauto|].
+    destruct ai_rest as [| ? ai_rest]; [by inversion Hlength_rest1|]. destruct ais_rest as [| ? ais_rest]; [by inversion Hlength_rest1'|].
+    iPrologue_both "Hprog" "Hsprog".
+    iMod (step_move_success_reg _ [SeqCtx] with "[$Hspec $Hj $HsPC $Hsi $Hs1 $Hs_t9]")
+      as "(Hj & HsPC & Hsi & Hs1 & Hs_t9)";
+      [eapply decode_encode_instrW_inv|iCorrectPC as_crtcls_end s_end|iContiguous_next Hcont_rest1' 2|auto..].
+    iApply (wp_move_success_reg with "[$HPC $Hi $Hr1 $Hr_t9]");
+      [eapply decode_encode_instrW_inv|iCorrectPC a_crtcls_end a_end|iContiguous_next Hcont_rest1 2|..].
+    iEpilogue_both "(HPC & Hi & Hr1 & Hr_t9)". iCombinePtrn.
+    iDestruct (big_sepM_insert _ _ r_t9 with "[$Hregs $Hr_t9]") as "Hregs";[apply lookup_delete|rewrite insert_delete !(insert_commute _ _ r_t9)// insert_insert].
+    iDestruct (big_sepM_insert _ _ r_t9 with "[$Hsegs $Hs_t9]") as "Hsegs";[apply lookup_delete|rewrite insert_delete insert_insert].
+    (* lea r_t1 offset_to_counter + length incr_instrs *)
+    assert ((a_move + (offset_to_counter + (length incr_instrs)))%a = Some linkc) as H_counter_offset1.
+    { revert Hlinkrestc H_counter_offset incr_length. clear. intros. solve_addr. }
+    assert ((s_move + (offset_to_counter + (length decr_instrs)))%a = Some linkc') as H_counter_offset1'.
+    { revert Hlinkrestc' H_counter_offset' decr_length. clear. intros. solve_addr. }
+    destruct ai_rest as [| ? ai_rest]; [by inversion Hlength_rest1|]. destruct ais_rest as [| ? ais_rest]; [by inversion Hlength_rest1'|].
+    iPrologue_both "Hprog" "Hsprog".
+    iMod (step_lea_success_z _ [SeqCtx] _ _ _ _ _ _ _ _ _ _ _ _ linkc' with "[$Hspec $Hj $HsPC $Hsi $Hs1]")
+      as "(Hj & HsPC & Hsi & Hs1)";
+      [eapply decode_encode_instrW_inv|iCorrectPC as_crtcls_end s_end|iContiguous_next Hcont_rest1' 3|assumption|done|auto..].
+    iApply (wp_lea_success_z _ _ _ _ _ _ _ _ _ _ _ _ _ linkc with "[$HPC $Hi $Hr1]");
+      [eapply decode_encode_instrW_inv|iCorrectPC a_crtcls_end a_end|iContiguous_next Hcont_rest1 3|assumption|done|..].
+    iEpilogue_both "(HPC & Hi & Hr1)". iCombinePtrn.
+
+    (* crtcls *)
+    iDestruct (contiguous_between_program_split with "Hprog") as
+        (ai_crtcls' ai_rest' a_crtcls_end') "(Hcrtcls' & Hprog & #Hcont)".
+    { epose proof (contiguous_between_incr_addr _ 4%nat _ _ _ Hcont_rest1 eq_refl).
+      eapply contiguous_between_app with (a1:=[_;_;_;_]). 2: eapply Hcont_rest1.
+      all: eauto. }
+    iDestruct "Hcont" as %(Hcont_crtcls2 & Hcont_rest2 & Heqapp2 & Hlink2).
+
+    iDestruct (contiguous_between_program_split with "Hsprog") as
+        (ais_crtcls' ais_rest' as_crtcls_end') "(Hscrtcls' & Hsprog & #Hcont)".
+    { epose proof (contiguous_between_incr_addr _ 4%nat _ _ _ Hcont_rest1' eq_refl).
+      eapply contiguous_between_app with (a1:=[_;_;_;_]). 2: eapply Hcont_rest1'.
+      all: eauto. }
+    iDestruct "Hcont" as %(Hcont_crtcls2' & Hcont_rest2' & Heqapp2' & Hlink2').
+
+    assert (a_crtcls_end <= f15)%a as Ha1_after_crtcls.
+    { eapply contiguous_between_middle_bounds'. apply Hcont_rest1. repeat constructor. }
+    assert (as_crtcls_end <= f16)%a as Ha1_after_crtcls'.
+    { eapply contiguous_between_middle_bounds'. apply Hcont_rest1'. repeat constructor. }
+
+    iApply (wp_wand with "[-]").
+    iApply (crtcls_spec with "[- $Hspec $Hj $HPC $HsPC $Hcrtcls' $Hscrtcls' $Hpc_b $Hpcs_b $Ha_entry $Hs_entry $Hr0 $Hs0 $Hregs $Hsegs $Hr1 $Hs1 $Hr2 $Hs2 $HnaI $Hinv_malloc]");
+      [| |apply Hcont_crtcls2|apply Hcont_crtcls2'|apply Hwb_malloc|apply Ha_entry|apply Hwb_malloc'|apply Hs_entry| | |auto|done|auto..].
+    { eapply isCorrectPC_range_restrict. apply Hvpc3. split; auto.
+      eapply contiguous_between_bounds. apply Hcont_rest2. }
+    { eapply isCorrectPC_range_restrict. apply Hvpc3'. split; auto.
+      eapply contiguous_between_bounds. apply Hcont_rest2'. }
+    { rewrite !dom_insert_L !dom_delete_L Hdom_r'. clear. set_solver-. }
+    { rewrite !dom_insert_L !dom_delete_L Hdom_s'. clear. set_solver-. }
+    2: { iIntros (?) "[ H | -> ]". iApply "H". iIntros (HC). congruence. }
+    iNext. iIntros "(Hj & HPC & Hcrtcls' & HsPC & Hscrtcls' & Hpc_b & Hpcs_b & Ha_entry & Hs_entry & HH)".
+    iDestruct "HH" as (b_cls' e_cls' Hbe_cls') "(Hr1 & Hs1 & Hbe_cls' & Hbes_cls' & Hr0 & Hs0 & Hr2 & Hs2 & HnaI & Hregs & Hsegs)".
+    iDestruct (big_sepL2_length with "Hprog") as %Hlength_rest2.
+    iDestruct (big_sepL2_length with "Hsprog") as %Hlength_rest2'.
+    (* register map cleanup *)
+    do 2 (repeat (rewrite (insert_commute _ _ r_t7);[|by auto]);rewrite insert_insert).
+    do 2 (repeat (rewrite (insert_commute _ _ r_t6);[|by auto]);rewrite insert_insert).
+    do 2 (repeat (rewrite (insert_commute _ _ r_t5);[|by auto]);rewrite insert_insert).
+    do 2 (repeat (rewrite (insert_commute _ _ r_t4);[|by auto]);rewrite insert_insert).
+    do 2 (repeat (rewrite (insert_commute _ _ r_t3);[|by auto]);rewrite insert_insert).
+
+    (* FINAL CLEANUP BEFORE RETURN *)
+    assert (isCorrectPC_range pc_p pc_b pc_e a_crtcls_end' a_end) as Hvpc4.
+    { eapply isCorrectPC_range_restrict. apply Hvpc3.
+      generalize (contiguous_between_bounds _ _ _ Hcont_rest2).
+      revert Ha1_after_malloc Ha1_after_crtcls Hlink2 Hlink1. clear; solve_addr. }
+    assert (isCorrectPC_range pcs_p pcs_b pcs_e as_crtcls_end' s_end) as Hvpc4'.
+    { eapply isCorrectPC_range_restrict. apply Hvpc3'.
+      generalize (contiguous_between_bounds _ _ _ Hcont_rest2').
+      revert Ha1_after_malloc' Ha1_after_crtcls' Hlink2' Hlink1'. clear; solve_addr. }
+
+    (* move r_t2 r_t10 *)
+    destruct ai_rest' as [| ? ai_rest']; [by inversion Hlength_rest2|].
+    pose proof (contiguous_between_cons_inv_first _ _ _ _ Hcont_rest2) as ->.
+    destruct ais_rest' as [| ? ais_rest']; [by inversion Hlength_rest2'|].
+    pose proof (contiguous_between_cons_inv_first _ _ _ _ Hcont_rest2') as ->.
+    destruct ai_rest' as [| ? ai_rest']; [by inversion Hlength_rest2|].
+    destruct ais_rest' as [| ? ais_rest']; [by inversion Hlength_rest2'|].
+    iPrologue_both "Hprog" "Hsprog".
+    rewrite !(insert_commute _ _ r_t10);auto.
+    iDestruct (big_sepM_delete _ _ r_t10 with "Hregs") as "[Hr_t10 Hregs]";[apply lookup_insert|].
+    iDestruct (big_sepM_delete _ _ r_t10 with "Hsegs") as "[Hs_t10 Hsegs]";[apply lookup_insert|].
+    iMod (step_move_success_reg _ [SeqCtx] with "[$Hspec $Hj $HsPC $Hsi $Hs2 $Hs_t10]")
+      as "(Hj & HsPC & Hsi & Hs2 & Hs_t10)";
+      [eapply decode_encode_instrW_inv|iCorrectPC as_crtcls_end' s_end|iContiguous_next Hcont_rest2' 0|auto..].
+    iApply (wp_move_success_reg with "[$HPC $Hi $Hr2 $Hr_t10]");
+      [eapply decode_encode_instrW_inv|iCorrectPC a_crtcls_end' a_end|iContiguous_next Hcont_rest2 0|..].
+    iEpilogue_both "(HPC & Hi & Hr2 & Hr_t10)". iCombinePtrn.
+    (* move r_t10 0 *)
+    destruct ai_rest' as [| ? ai_rest']; [by inversion Hlength_rest2|]. destruct ais_rest' as [| ? ais_rest']; [by inversion Hlength_rest2'|].
+    iPrologue_both "Hprog" "Hsprog".
+    iMod (step_move_success_z _ [SeqCtx] with "[$Hspec $Hj $HsPC $Hsi $Hs_t10]")
+      as "(Hj & HsPC & Hsi & Hs_t10)";
+      [eapply decode_encode_instrW_inv|iCorrectPC as_crtcls_end' s_end|iContiguous_next Hcont_rest2' 1|auto..].
+    iApply (wp_move_success_z with "[$HPC $Hi $Hr_t10]");
+      [eapply decode_encode_instrW_inv|iCorrectPC a_crtcls_end' a_end|iContiguous_next Hcont_rest2 1|..].
+    iEpilogue_both "(HPC & Hi & Hr_t10)". iCombinePtrn.
+    iDestruct (big_sepM_insert _ _ r_t10 with "[$Hregs $Hr_t10]") as "Hregs";[apply lookup_delete|rewrite insert_delete insert_insert].
+    iDestruct (big_sepM_insert _ _ r_t10 with "[$Hsegs $Hs_t10]") as "Hsegs";[apply lookup_delete|rewrite insert_delete insert_insert].
+    (* move r_t8 0 *)
+    iDestruct (big_sepM_delete _ _ r_t8 with "Hregs") as "[Hr_t8 Hregs]".
+    { repeat (rewrite lookup_insert_ne;[|by auto]). apply lookup_insert. }
+    iDestruct (big_sepM_delete _ _ r_t8 with "Hsegs") as "[Hs_t8 Hsegs]".
+    { repeat (rewrite lookup_insert_ne;[|by auto]). apply lookup_insert. }
+    destruct ai_rest' as [| ? ai_rest']; [by inversion Hlength_rest2|]. destruct ais_rest' as [| ? ais_rest']; [by inversion Hlength_rest2'|].
+    iPrologue_both "Hprog" "Hsprog".
+    iMod (step_move_success_z _ [SeqCtx] with "[$Hspec $Hj $HsPC $Hsi $Hs_t8]")
+      as "(Hj & HsPC & Hsi & Hs_t8)";
+      [eapply decode_encode_instrW_inv|iCorrectPC as_crtcls_end' s_end|iContiguous_next Hcont_rest2' 2|auto..].
+    iApply (wp_move_success_z with "[$HPC $Hi $Hr_t8]");
+      [eapply decode_encode_instrW_inv|iCorrectPC a_crtcls_end' a_end|iContiguous_next Hcont_rest2 2|..].
+    iEpilogue_both "(HPC & Hi & Hr_t8)". iCombinePtrn.
+    iDestruct (big_sepM_insert _ _ r_t8 with "[$Hregs $Hr_t8]") as "Hregs";[apply lookup_delete|rewrite insert_delete].
+    iDestruct (big_sepM_insert _ _ r_t8 with "[$Hsegs $Hs_t8]") as "Hsegs";[apply lookup_delete|rewrite insert_delete].
+    (* move r_t9 0 *)
+    iDestruct (big_sepM_delete _ _ r_t9 with "Hregs") as "[Hr_t9 Hregs]".
+    { repeat (rewrite lookup_insert_ne;[|by auto]). apply lookup_insert. }
+    iDestruct (big_sepM_delete _ _ r_t9 with "Hsegs") as "[Hs_t9 Hsegs]".
+    { repeat (rewrite lookup_insert_ne;[|by auto]). apply lookup_insert. }
+    destruct ai_rest' as [| ? ai_rest']; [by inversion Hlength_rest2|]. destruct ais_rest' as [| ? ais_rest']; [by inversion Hlength_rest2'|].
+    iPrologue_both "Hprog" "Hsprog".
+    iMod (step_move_success_z _ [SeqCtx] with "[$Hspec $Hj $HsPC $Hsi $Hs_t9]")
+      as "(Hj & HsPC & Hsi & Hs_t9)";
+      [eapply decode_encode_instrW_inv|iCorrectPC as_crtcls_end' s_end|iContiguous_next Hcont_rest2' 3|auto..].
+    iApply (wp_move_success_z with "[$HPC $Hi $Hr_t9]");
+      [eapply decode_encode_instrW_inv|iCorrectPC a_crtcls_end' a_end|iContiguous_next Hcont_rest2 3|..].
+    iEpilogue_both "(HPC & Hi & Hr_t9)". iCombinePtrn.
+    iDestruct (big_sepM_insert _ _ r_t9 with "[$Hregs $Hr_t9]") as "Hregs";[apply lookup_delete|rewrite insert_delete].
+    iDestruct (big_sepM_insert _ _ r_t9 with "[$Hsegs $Hs_t9]") as "Hsegs";[apply lookup_delete|rewrite insert_delete].
+
+    (* WE WILL NOW PREPARE THΕ JUMP *)
+    iCombine "Hbes_cls" "Hbes_cls'" as "Hbes_cls".
+    iCombine "Hbe_cls'" "Hbes_cls" as "Hbe_cls'".
+    iCombine "Hbe_cls" "Hbe_cls'" as "Hbe_cls".
+    iDestruct (na_inv_alloc logrel_nais _ count_clsN with "Hbe_cls") as ">#Hcls_inv".
+
+    (* in preparation of jumping, we allocate the counter invariant *)
+    (* in this closure creation, the two programs have the same address as the counter. This is not necessary however! *)
+    iDestruct (inv_alloc countN _ (offset_counter_inv offset b_cell b_cell) with "[Hb_cell Hb_scell]") as ">#Hcounter_inv".
+    { iNext. rewrite /offset_counter_inv. iExists 0. assert ((0%nat + offset)%Z = offset)%Z as ->;[clear;lia|]. iFrame. }
+    (* we also allocate a non atomic invariant for the environment table *)
+    (* iMod (na_inv_alloc logrel_nais _ count_env *)
+    (*                    (pc_b ↦ₐ WCap (RO,b_link,e_link,a_link) ∗ a_entry' ↦ₐ fail_cap)%I *)
+    (*         with "[$Ha_entry' $Hpc_b]") as "#Henv". *)
+
+    (* jmp *)
+    destruct ai_rest' as [| ? ai_rest']; [|by inversion Hlength_rest2]. destruct ais_rest' as [| ? ais_rest']; [|by inversion Hlength_rest2'].
+    iPrologue_both "Hprog" "Hsprog".
+    iMod (step_jmp_success _ [SeqCtx] with "[$Hspec $Hj $HsPC $Hsi $Hs0]")
+      as "(Hj & HsPC & Hsi & Hs0)";
+      [apply decode_encode_instrW_inv|iCorrectPC as_crtcls_end' s_end|auto..].
+    iApply (wp_jmp_success with "[$HPC $Hi $Hr0]");
+      [apply decode_encode_instrW_inv|iCorrectPC a_crtcls_end' a_end|..].
+
+    (* the current state of registers is valid *)
+    iAssert (interp (WCap E b_cls e_cls b_cls,WCap E b_cls e_cls b_cls))%I as "#Hvalid_cls".
+    { iApply (incr_offset_closure_valid with "Hspec Hcounter_inv Hincr Hcls_inv");auto.
+      apply Hvpc_counter. apply Hvpc_counter'. apply Hcont_restc. apply Hcont_restc'. solve_ndisj. }
+
+    iAssert (interp (WCap E b_cls' e_cls' b_cls',WCap E b_cls' e_cls' b_cls'))%I as "#Hvalid_cls'".
+    { iApply (read_offset_closure_valid with "Hspec Hcounter_inv Hread Hcls_inv");auto.
+      apply Hcont_restc. apply Hcont_restc'. apply Hvpc_counter. apply Hvpc_counter'.
+      apply Hcont_incr. apply Hcont_decr. solve_ndisj. }
+
+    unshelve iPoseProof ("Hr_valid" $! r_t0 _ _ _ Hr0 Hs0) as "#Hr0_valid". done.
+
+    (* either we fail, or we use the continuation in rt0 *)
+    iDestruct (jmp_or_fail_spec with "Hspec Hr0_valid") as "Hcont".
+    destruct (decide (isCorrectPC (updatePcPerm r0))).
+    2 : { iEpilogue_both "(HPC & Hi & Hr0)". iApply "Hcont". iFrame "HPC". iIntros (Hcontr);done. }
+    iDestruct "Hcont" as (p b e ? Heq) "#Hcont".
+    simplify_eq.
+
+    (* prepare the continuation *)
+    iEpilogue_both "(HPC & Hi & Hr0)". iCombinePtrn.
+
+    (* Put the registers back in the map *)
+    iDestruct (big_sepM_insert with "[$Hregs $Hr2]") as "Hregs".
+    { repeat (rewrite lookup_insert_ne //;[]). rewrite lookup_delete //. }
+    iDestruct (big_sepM_insert with "[$Hregs $Hr1]") as "Hregs".
+    { repeat (rewrite lookup_insert_ne //;[]). rewrite lookup_delete_ne //.
+      repeat (rewrite lookup_insert_ne //;[]). apply lookup_delete. }
+    iDestruct (big_sepM_insert with "[$Hregs $Hr0]") as "Hregs".
+    { repeat (rewrite lookup_insert_ne //;[]). rewrite lookup_delete_ne //.
+      repeat (rewrite lookup_insert_ne //;[]). rewrite lookup_delete_ne // lookup_delete //. }
+    iDestruct (big_sepM_insert with "[$Hregs $HPC]") as "Hregs".
+    { repeat (rewrite lookup_insert_ne //;[]). rewrite lookup_delete_ne //.
+      repeat (rewrite lookup_insert_ne //;[]). do 2 rewrite lookup_delete_ne //.
+      apply lookup_delete. }
+    iDestruct (big_sepM_insert with "[$Hsegs $Hs2]") as "Hsegs".
+    { repeat (rewrite lookup_insert_ne //;[]). rewrite lookup_delete //. }
+    iDestruct (big_sepM_insert with "[$Hsegs $Hs1]") as "Hsegs".
+    { repeat (rewrite lookup_insert_ne //;[]). rewrite lookup_delete_ne //.
+      repeat (rewrite lookup_insert_ne //;[]). apply lookup_delete. }
+    iDestruct (big_sepM_insert with "[$Hsegs $Hs0]") as "Hsegs".
+    { repeat (rewrite lookup_insert_ne //;[]). rewrite lookup_delete_ne //.
+      repeat (rewrite lookup_insert_ne //;[]). rewrite lookup_delete_ne // lookup_delete //. }
+    iDestruct (big_sepM_insert with "[$Hsegs $HsPC]") as "Hsegs".
+    { repeat (rewrite lookup_insert_ne //;[]). rewrite lookup_delete_ne //.
+      repeat (rewrite lookup_insert_ne //;[]). do 2 rewrite lookup_delete_ne //.
+      apply lookup_delete. }
+
+    do 2 (repeat (rewrite -(delete_insert_ne _ r_t2) //;[]);rewrite insert_delete).
+    do 2 (repeat (rewrite -(delete_insert_ne _ r_t1) //;[]);rewrite insert_delete).
+    do 2 (repeat (rewrite -(delete_insert_ne _ r_t0) //;[]);rewrite insert_delete).
+    do 2 (repeat (rewrite -(delete_insert_ne _ PC) //;[]);rewrite insert_delete).
+
+    rewrite -(insert_insert _ PC (updatePcPerm s0) (WInt 0%Z))  -(insert_insert _ PC _ (WInt 0%Z)).
+
+    match goal with |- context [ ([∗ map] k↦y ∈ <[PC:=_]> ?r, _)%I ] => set r'' := r end.
+    match goal with |- context [ ([∗ map] k↦y ∈ <[PC:=updatePcPerm s0]> ?r, _)%I ] => set s'' := r end.
+    iDestruct (interp_eq with "Hr0_valid") as %<-.
+    iAssert (full_map (r'',s'')) as %Hr''_full.
+    { rewrite /full_map. iIntros (rr). iPureIntro. split.
+      - rewrite elem_of_gmap_dom /r''.
+        rewrite !dom_insert_L regmap_full_dom //.
+        generalize (all_registers_s_correct rr). clear; set_solver.
+      - rewrite elem_of_gmap_dom /s''.
+        rewrite !dom_insert_L regmap_full_dom //.
+        generalize (all_registers_s_correct rr). clear; set_solver. }
+    iSpecialize ("Hcont" $! (r'',s'') with "[$Hj $Hregs $Hsegs $HnaI]").
+    { rewrite /interp_reg. iSplit; [iPureIntro; apply Hr''_full|].
+      iIntros (rr v1 v2 Hrr Hv1s Hv2s). simpl. rewrite /r'' /s'' in Hv1s, Hv2s.
+      repeat (
+      match goal with H : context [ <[?r := _]> _ ] |- _ =>
+                      consider_next_reg_both1 rr r Hv1s Hv2s; [simplify_eq; try done; by rewrite (fixpoint_interp1_eq (WInt 0%Z, WInt 0%Z))|]
+      end ).
+      simplify_eq.
+      by unshelve iSpecialize ("Hr_valid" $! rr _ _ n Hv1s Hv2s).
+    }
+    (* apply the continuation *)
+    iDestruct "Hcont" as "[_ Hcallback_now]".
+    iApply wp_wand_l. iFrame "Hcallback_now".
+    iIntros (v) "Hφ". iIntros (Hne).
+    iDestruct ("Hφ" $! Hne) as (r0) "(Hfull & Hregs & Hna)".
+    iExists r0. iFrame.
+  Qed.
 
 End counter_example_preamble.
